$$
\begin{gather}
(x+y)^1=x+y \\
(x+y)^{2}=x^{2}+2xy+y^{2} \\
(x+y)^{3}=x^{3}+3x^{2}y+3xy^{2}+y^{3} \\
(x+y)^4=x^4+4x^{3}y+6x^{2}y^{2}+4xy^{3}+y^4 \\
(x+y)(x+y)(x+y)(x+y)(x+y)= x^5+5x^4y+10x^{3}y^{2}+10y^{3}x^{2}+5y^4x+y^5
\end{gather}
$$
$$
\begin{align} \\
 1 \\
1    & 1 \\
1 &  2 &   1 \\
  1 &  3 &   3 &   1 \\
1  & 4  & 6   & 4  & 1 \\
1 & 5 & 10 & 10 & 5 & 1 \\
1 & 6 & 15 & 20 & 15 &6 &  1

\end{align}
$$
$$
x^6+6x^5y+15x^4y^2+20x^3y^3+15x^{2}y^4+6xy^5+y^6
$$
$$
(\sqrt{ 2 }+1)^6=\sqrt{ 2 }^6+6\sqrt{ 2 }^5+15\sqrt{ 2 }^4+20\sqrt{ 2 }^3+15\sqrt{ 2 }^{2}+6\sqrt{ 2 }+1
$$
$$
8+24\sqrt{ 2 }+60+40\sqrt{ 2 }+30
+6\sqrt{ 2 }+1$$
$$
99+70\sqrt{ 2 }
$$
$$
\begin{multline} \framebox[.65\columnwidth]{A}\\ \framebox[.5\columnwidth]{B}\\ \shoveright{\framebox[.55\columnwidth]{C}}\\ \framebox[.65\columnwidth]{D} \end{multline}
$$
$$
\begin{equation}
\begin{split} H_c&=\frac{1}{2n}
\sum^n_{l=0}(-1)^{l}(n-{l})^{p-2} \sum_{l _1+\dots+ l _p=l}\prod^p_{i=1} \binom{n_i}{l _i}\\ &\quad\cdot[(n-l )-(n_i-l _i)]^{n_i-l _i}\cdot \Bigl[(n-l )^2-\sum^p_{j=1}(n_i-l _i)^2\Bigr]. \end{split}
\end{equation}
$$
$$

$$